Substitution must act on free variables, not bound ones

ecoop17/dot_storeless_subst_aux.v
@@ -9,7 +9,7 @@ Require Import tactics.
 (*******************)
 (* Infrastructure for total parallel substitution on locally closed terms *)
 
-Definition wf {A} (G : list A) T := closed 0 (length G) T.
+Definition wf {A} (G : list A) T := closed (length G) 0 T.
 
 Ltac beq_nat :=
   match goal with
@@ -34,12 +34,33 @@ Lemma dms_closed_upgrade: forall i k k1 v,
 Proof. unmut_lemma closed_upgrade_rec. Qed.
 Hint Resolve dm_closed_upgrade tm_closed_upgrade vr_closed_upgrade dms_closed_upgrade.
 
+Lemma vr_closed_upgrade_gh: forall i i1 k v,
+  vr_closed i k v -> i <= i1 -> vr_closed i1 k v.
+Proof. unmut_lemma closed_upgrade_gh_rec. Qed.
+Lemma tm_closed_upgrade_gh: forall i i1 k v,
+  tm_closed i k v -> i <= i1 -> tm_closed i1 k v.
+Proof. unmut_lemma closed_upgrade_gh_rec. Qed.
+Lemma dm_closed_upgrade_gh: forall i i1 k v,
+  dm_closed i k v -> i <= i1 -> dm_closed i1 k v.
+Proof. unmut_lemma closed_upgrade_gh_rec. Qed.
+Lemma dms_closed_upgrade_gh: forall i i1 k v,
+  dms_closed i k v -> i <= i1 -> dms_closed i1 k v.
+Proof. unmut_lemma closed_upgrade_gh_rec. Qed.
+Hint Resolve vr_closed_upgrade_gh closed_upgrade_gh tm_closed_upgrade_gh dm_closed_upgrade_gh dms_closed_upgrade_gh : upgrade.
+
 Lemma env_closed_upgrade: forall i k k1 env,
   Forall (vr_closed i k) env ->
   k <= k1 ->
   Forall (vr_closed i k1) env.
 Proof. eauto using Forall_impl. Qed.
 Hint Resolve env_closed_upgrade.
+
+Lemma env_closed_upgrade_gh: forall i i1 k env,
+  Forall (vr_closed i k) env ->
+  i <= i1 ->
+  Forall (vr_closed i1 k) env.
+Proof. eauto using Forall_impl with upgrade. Qed.
+Hint Resolve env_closed_upgrade_gh : upgrade.
 
 Hint Constructors Forall.
 
@@ -88,66 +109,66 @@ Admitted.
 
 Require Import dot_monads.
 
-Fixpoint vr_subst_all_k k (env: list vr) (v: vr) { struct v }: option vr :=
+Fixpoint vr_subst_all (env: list vr) (v: vr) { struct v }: option vr :=
   match v with
-    | VarF x => ret (VarF x)
-    | VarB x => index x env
+    | VarF x => index x env
+    | VarB x => ret (VarB x)
     | VObj dms =>
-      dms' <- dms_subst_all_k (S k) (VarB k :: env) dms;
+      dms' <- dms_subst_all env dms;
       ret (VObj dms')
   end
-with subst_all_k k (env: list vr) (T: ty) { struct T }: option ty :=
+with subst_all (env: list vr) (T: ty) { struct T }: option ty :=
   match T with
     | TTop        => ret TTop
     | TBot        => ret TBot
     | TSel v1 l     =>
-      v1' <- vr_subst_all_k k env v1;
+      v1' <- vr_subst_all env v1;
       ret (TSel v1' l)
     | TFun l T1 T2  =>
-      T1' <- subst_all_k k env T1;
-      T2' <- subst_all_k (S k) (VarB k :: env) T2;
+      T1' <- subst_all env T1;
+      T2' <- subst_all env T2;
       ret (TFun l T1' T2')
     | TMem l T1 T2  =>
-      T1' <- subst_all_k k env T1;
-      T2' <- subst_all_k k env T2;
+      T1' <- subst_all env T1;
+      T2' <- subst_all env T2;
       ret (TMem l T1' T2')
     | TBind T1    =>
-      T1' <- subst_all_k (S k) (VarB k :: env) T1;
+      T1' <- subst_all env T1;
       ret (TBind T1')
     | TAnd T1 T2  =>
-      T1' <- subst_all_k k env T1;
-      T2' <- subst_all_k k env T2;
+      T1' <- subst_all env T1;
+      T2' <- subst_all env T2;
       ret (TAnd T1' T2')
     | TOr T1 T2   =>
-      T1' <- subst_all_k k env T1;
-      T2' <- subst_all_k k env T2;
+      T1' <- subst_all env T1;
+      T2' <- subst_all env T2;
       ret (TOr T1' T2')
   end
-with tm_subst_all_k k (env: list vr) (t: tm) { struct t }: option tm :=
+with tm_subst_all (env: list vr) (t: tm) { struct t }: option tm :=
    match t with
-     | tvar v => v' <- vr_subst_all_k k env v; ret (tvar v')
+     | tvar v => v' <- vr_subst_all env v; ret (tvar v')
      | tapp t1 l t2 =>
-       t1' <- tm_subst_all_k k env t1;
-       t2' <- tm_subst_all_k k env t2;
+       t1' <- tm_subst_all env t1;
+       t2' <- tm_subst_all env t2;
        ret (tapp t1' l t2')
    end
-with dm_subst_all_k k (env: list vr) (d: dm) { struct d }: option dm :=
+with dm_subst_all (env: list vr) (d: dm) { struct d }: option dm :=
    match d with
      | dfun T1 T2 t2 =>
-       T1' <- subst_all_k k env T1;
-       T2' <- subst_all_k (S k) (VarB k :: env) T2;
-       t2' <- tm_subst_all_k (S k) (VarB k :: env) t2;
+       T1' <- subst_all env T1;
+       T2' <- subst_all env T2;
+       t2' <- tm_subst_all env t2;
        ret (dfun T1' T2' t2')
      | dty T1 =>
-       T1' <- subst_all_k k env T1;
+       T1' <- subst_all env T1;
        ret (dty T1')
    end
-with dms_subst_all_k k (env: list vr) (ds: dms) { struct ds }: option dms :=
+with dms_subst_all (env: list vr) (ds: dms) { struct ds }: option dms :=
    match ds with
      | dnil => ret dnil
      | dcons d ds =>
-       d'  <- dm_subst_all_k k env d;
-       ds' <- dms_subst_all_k k env ds;
+       d'  <- dm_subst_all env d;
+       ds' <- dms_subst_all env ds;
        ret (dcons d' ds')
    end.
 
@@ -168,54 +189,54 @@ Proof. eauto using Forall_map. Qed.
 Hint Resolve dms_to_env_closed.
 
 Lemma subst_all_nonTot_res_closed_rec:
-  (forall v, forall i k env, Forall (vr_closed i k) env -> vr_closed i (length env) v ->
-          exists v', vr_subst_all_k k env v = Some v' /\
+  (forall v, forall i k env, Forall (vr_closed i k) env -> vr_closed (length env) k v ->
+          exists v', vr_subst_all env v = Some v' /\
                 vr_closed i k v') /\
-  (forall T, forall i k env, Forall (vr_closed i k) env -> closed i (length env) T ->
-          exists T', subst_all_k k env T = Some T' /\
+  (forall T, forall i k env, Forall (vr_closed i k) env -> closed (length env) k T ->
+          exists T', subst_all env T = Some T' /\
                 closed i k T') /\
-  (forall t, forall i k env, Forall (vr_closed i k) env -> tm_closed i (length env) t ->
-          exists t', tm_subst_all_k k env t = Some t' /\
+  (forall t, forall i k env, Forall (vr_closed i k) env -> tm_closed (length env) k t ->
+          exists t', tm_subst_all env t = Some t' /\
                 tm_closed i k t') /\
-  (forall d, forall i k env, Forall (vr_closed i k) env -> dm_closed i (length env) d ->
-          exists d', dm_subst_all_k k env d = Some d' /\
+  (forall d, forall i k env, Forall (vr_closed i k) env -> dm_closed (length env) k d ->
+          exists d', dm_subst_all env d = Some d' /\
                 dm_closed i k d') /\
-  (forall d, forall i k env, Forall (vr_closed i k) env -> dms_closed i (length env) d ->
-          exists d', dms_subst_all_k k env d = Some d' /\
+  (forall d, forall i k env, Forall (vr_closed i k) env -> dms_closed (length env) k d ->
+          exists d', dms_subst_all env d = Some d' /\
                 dms_closed i k d').
 Proof.
   apply syntax_mutind; simpl; intros; inverts_closed;
     repeat
       match goal with
-      | Hind : context [ ?f _ _ ?s ] |- context [ match ?f ?k ?env ?s with _ => _ end ] =>
+      | Hind : context [ ?f _ ?s ] , Hcl : _ (length _) ?k ?s |- context [ match ?f ?env ?s with _ => _ end ] =>
         lets (? & -> & ?): Hind i k env ___
       end;
     eauto using index_Forall.
 Qed.
 
 Lemma vr_subst_all_nonTot_res_closed:
-  (forall v i k env, Forall (vr_closed i k) env -> forall (Hcl: vr_closed i (length env) v),
-          exists v', vr_subst_all_k k env v = Some v' /\
+  (forall v i k env, Forall (vr_closed i k) env -> forall (Hcl: vr_closed (length env) k v),
+          exists v', vr_subst_all env v = Some v' /\
                 vr_closed i k v').
 Proof. unmut_lemma subst_all_nonTot_res_closed_rec. Qed.
 Lemma subst_all_nonTot_res_closed:
-  (forall T i k env, Forall (vr_closed i k) env -> forall (Hcl: closed i (length env) T),
-          exists T', subst_all_k k env T = Some T' /\
+  (forall T i k env, Forall (vr_closed i k) env -> forall (Hcl: closed (length env) k T),
+          exists T', subst_all env T = Some T' /\
                 closed i k T').
 Proof. unmut_lemma subst_all_nonTot_res_closed_rec. Qed.
 Lemma tm_subst_all_nonTot_res_closed:
-  (forall t i k env, Forall (vr_closed i k) env -> forall (Hcl: tm_closed i (length env) t),
-          exists t', tm_subst_all_k k env t = Some t' /\
+  (forall t i k env, Forall (vr_closed i k) env -> forall (Hcl: tm_closed (length env) k t),
+          exists t', tm_subst_all env t = Some t' /\
                 tm_closed i k t').
 Proof. unmut_lemma subst_all_nonTot_res_closed_rec. Qed.
 Lemma dm_subst_all_nonTot_res_closed:
-  (forall d i k env, Forall (vr_closed i k) env -> forall (Hcl: dm_closed i (length env) d),
-          exists d', dm_subst_all_k k env d = Some d' /\
+  (forall d i k env, Forall (vr_closed i k) env -> forall (Hcl: dm_closed (length env) k d),
+          exists d', dm_subst_all env d = Some d' /\
                 dm_closed i k d').
 Proof. unmut_lemma subst_all_nonTot_res_closed_rec. Qed.
 Lemma dms_subst_all_nonTot_res_closed:
-  (forall d i k env, Forall (vr_closed i k) env -> forall (Hcl: dms_closed i (length env) d),
-          exists d', dms_subst_all_k k env d = Some d' /\
+  (forall d i k env, Forall (vr_closed i k) env -> forall (Hcl: dms_closed (length env) k d),
+          exists d', dms_subst_all env d = Some d' /\
                 dms_closed i k d').
 Proof. unmut_lemma subst_all_nonTot_res_closed_rec. Qed.
 Hint Resolve
@@ -225,18 +246,18 @@ Hint Resolve
      dm_subst_all_nonTot_res_closed
      dms_subst_all_nonTot_res_closed.
 
-Definition evalToSome env e v l k j :=
-  (exists t', tm_subst_all_k l (map VObj env) e = Some t' /\ steps t' v j) /\ irred v /\ j <= k.
+Definition evalToSome env e v k j :=
+  (exists t', tm_subst_all (map VObj env) e = Some t' /\ steps t' v j) /\ irred v /\ j <= k.
 
 Lemma evalToSomeRes_closed: forall env e v n k j l,
-    evalToSome env e v k n j ->
-    tm_closed 0 l e ->
+    evalToSome env e v n j ->
+    tm_closed l 0 e ->
     length env = l ->
-    Forall (dms_closed 0 (S k)) env ->
-    tm_closed 0 k v.
+    Forall (dms_closed k 1) env ->
+    tm_closed k 0 v.
 Proof.
   unfold evalToSome; intros; subst;
-    assert (exists t', tm_subst_all_k k (map VObj env) e = Some t' /\ tm_closed 0 k t')
+    assert (exists t', tm_subst_all (map VObj env) e = Some t' /\ tm_closed k 0 t')
     by (eapply tm_subst_all_nonTot_res_closed; try rewrite map_length; eauto); ev;
       optFuncs_det;
       eauto using steps_closed.
@@ -248,14 +269,14 @@ Hint Resolve evalToSomeRes_closed.
    We must first prove that substitution leaves them unchnaged. *)
 
 (* Define what's an identity substitution, through the required property (rather than through an inductive type). *)
-Definition vr_env_id xs := forall n, n < length xs -> index n xs = Some (VarB n).
+Definition vr_env_id xs := forall n, n < length xs -> index n xs = Some (VarF n).
 
 (* Allow proving vr_env_id. These lemmas could probably be the constructors for
    an inductive characterization. *)
 Lemma nil_vr_env_id: vr_env_id [].
 Proof. unfold vr_env_id; simpl; easy. Qed.
 
-Lemma cons_vr_env_id: forall env, vr_env_id env -> vr_env_id (VarB (length env) :: env).
+Lemma cons_vr_env_id: forall env, vr_env_id env -> vr_env_id (VarF (length env) :: env).
 Proof. unfold vr_env_id; simpl; intros; case_match; beq_nat; subst; auto. Qed.
 
 Hint Resolve nil_vr_env_id cons_vr_env_id.
@@ -263,39 +284,39 @@ Hint Resolve nil_vr_env_id cons_vr_env_id.
 (* Prove that an identity substitution is also an identity when lifted to our
    language syntax. *)
 Lemma subst_closed_id_rec:
-  (forall v i env, vr_env_id env -> vr_closed i (length env) v ->
-          vr_subst_all_k (length env) env v = Some v) /\
-  (forall T i env, vr_env_id env -> closed i (length env) T ->
-          subst_all_k (length env) env T = Some T) /\
-  (forall t i env, vr_env_id env -> tm_closed i (length env) t ->
-          tm_subst_all_k (length env) env t = Some t) /\
-  (forall d i env, vr_env_id env -> dm_closed i (length env) d ->
-          dm_subst_all_k (length env) env d = Some d) /\
-  (forall d i env, vr_env_id env -> dms_closed i (length env) d ->
-          dms_subst_all_k (length env) env d = Some d).
+  (forall v i env, vr_env_id env -> vr_closed (length env) i v ->
+          vr_subst_all env v = Some v) /\
+  (forall T i env, vr_env_id env -> closed (length env) i T ->
+          subst_all env T = Some T) /\
+  (forall t i env, vr_env_id env -> tm_closed (length env) i t ->
+          tm_subst_all env t = Some t) /\
+  (forall d i env, vr_env_id env -> dm_closed (length env) i d ->
+          dm_subst_all env d = Some d) /\
+  (forall d i env, vr_env_id env -> dms_closed (length env) i d ->
+          dms_subst_all env d = Some d).
 Proof.
   apply syntax_mutind; simpl; intros; inverts_closed;
     repeat
       match goal with
-      | Hind : context [ ?f _ _ ?s ] |- context [ match ?f ?k ?env ?s with _ => _ end ] =>
+      | Hind : context [ ?f _ ?s ], Hcl : _ (length _) ?i ?s  |- context [ match ?f ?env ?s with _ => _ end ] =>
         lets ->: Hind i env ___
       end;
     eauto.
 Qed.
 
-Lemma tm_subst_closed_id: forall t i env, tm_closed i (length env) t -> vr_env_id env -> tm_subst_all_k (length env) env t = Some t.
+Lemma tm_subst_closed_id: forall t i env, tm_closed (length env) i t -> vr_env_id env -> tm_subst_all env t = Some t.
 Proof. unmut_lemma subst_closed_id_rec. Qed.
 
 Lemma tm_subst_closed_id': forall t i l env,
     l = length env ->
-    tm_closed i l t -> vr_env_id env -> tm_subst_all_k l env t = Some t.
+    tm_closed l i t -> vr_env_id env -> tm_subst_all env t = Some t.
 Proof. intros; subst; eauto using tm_subst_closed_id. Qed.
 
-Lemma tm_subst_closed_id_nil: forall t i, tm_closed i 0 t -> tm_subst_all_k 0 [] t = Some t.
+Lemma tm_subst_closed_id_nil: forall t i, tm_closed 0 i t -> tm_subst_all [] t = Some t.
 Proof. eauto using tm_subst_closed_id'. Qed.
 Hint Resolve tm_subst_closed_id_nil.
 
 Hint Constructors steps.
 
-Lemma vl_evalToSome_self: forall v n i, irred v -> tm_closed i 0 v -> evalToSome [] v v 0 n 0.
+Lemma vl_evalToSome_self: forall v n i, irred v -> tm_closed 0 i v -> evalToSome [] v v n 0.
 Proof. unfold evalToSome; intuition eauto. Qed.
